LeanSAT/Reflect/BVExpr/BitBlast/Impl/ZeroExtend.lean
@@ -1,0 +1,88 @@
+import LeanSAT.Reflect.BVExpr.Basic
+import LeanSAT.AIG
+
+namespace BVExpr
+namespace bitblast
+
+structure ZeroExtendTarget (aig : AIG BVBit) (newWidth : Nat) where
+  w : Nat
+  stream : AIG.RefStream aig w
+
+def blastZeroExtend (aig : AIG BVBit) (target : ZeroExtendTarget aig newWidth)
+    : AIG.RefStreamEntry BVBit newWidth :=
+  let ⟨width, input⟩ := target
+  go aig width input newWidth 0 (by omega) .empty
+where
+  go (aig : AIG BVBit) (w : Nat) (input : AIG.RefStream aig w) (newWidth : Nat) (curr : Nat) (hcurr : curr ≤ newWidth)
+      (s : AIG.RefStream aig curr) : AIG.RefStreamEntry BVBit newWidth :=
+    if hcurr1:curr < newWidth then
+      if hcurr2:curr < w then
+        let s := s.pushRef (input.getRef curr hcurr2)
+        go aig w input newWidth (curr + 1) (by omega) s
+      else
+        let res := aig.mkConstCached false
+        let aig := res.aig
+        let zeroRef := res.ref
+        have hcast := by
+          dsimp [aig, res]
+          apply AIG.LawfulOperator.le_size (f := AIG.mkConstCached)
+        let input := input.cast hcast
+        let s := s.cast hcast
+        let s := s.pushRef zeroRef
+        go aig w input newWidth (curr + 1) (by omega) s
+    else
+      have hcurr : curr = newWidth := by omega
+      ⟨aig, hcurr ▸ s⟩
+termination_by newWidth - curr
+
+namespace blastZeroExtend
+
+theorem go_le_size (aig : AIG BVBit) (w : Nat) (input : AIG.RefStream aig w) (newWidth curr : Nat)
+    (hcurr : curr ≤ newWidth) (s : AIG.RefStream aig curr)
+    : aig.decls.size ≤ (go aig w input newWidth curr hcurr s).aig.decls.size := by
+  unfold go
+  split
+  . dsimp
+    split
+    . refine Nat.le_trans ?_ (by apply go_le_size)
+      omega
+    . refine Nat.le_trans ?_ (by apply go_le_size)
+      apply AIG.LawfulOperator.le_size (f := AIG.mkConstCached)
+  . simp
+termination_by newWidth - curr
+
+theorem go_decl_eq (aig : AIG BVBit) (w : Nat) (input : AIG.RefStream aig w) (newWidth curr : Nat)
+    (hcurr : curr ≤ newWidth) (s : AIG.RefStream aig curr)
+    : ∀ (idx : Nat) (h1) (h2),
+       (go aig w input newWidth curr hcurr s).aig.decls[idx]'h2 = aig.decls[idx]'h1 := by
+  generalize hgo : go aig w input newWidth curr hcurr s = res
+  unfold go at hgo
+  split at hgo
+  . dsimp at hgo
+    split at hgo
+    . rw [← hgo]
+      intro idx h1 h2
+      rw [go_decl_eq]
+    . rw [← hgo]
+      intro idx h1 h2
+      rw [go_decl_eq]
+      rw [AIG.LawfulOperator.decl_eq (f := AIG.mkConstCached)]
+      apply AIG.LawfulOperator.lt_size_of_lt_aig_size (f := AIG.mkConstCached)
+      assumption
+  . simp [← hgo]
+termination_by newWidth - curr
+
+end blastZeroExtend
+
+instance : AIG.LawfulStreamOperator BVBit ZeroExtendTarget blastZeroExtend where
+  le_size := by
+    intros
+    unfold blastZeroExtend
+    apply blastZeroExtend.go_le_size
+  decl_eq := by
+    intros
+    unfold blastZeroExtend
+    apply blastZeroExtend.go_decl_eq
+
+end bitblast
+end BVExpr
